Updates

generic/Zeta.Generic.Global.fsti
@@ -3,6 +3,8 @@ module Zeta.Generic.Global
 open FStar.Seq
 open Zeta.SeqAux
 open Zeta.SSeq
+open Zeta.IdxFn
+open Zeta.SIdxFn
 open Zeta.Interleave
 open Zeta.Time
 open Zeta.MultiSetHashDomain
@@ -10,6 +12,7 @@ open Zeta.GenericVerifier
 open Zeta.Generic.Thread
 
 module S = FStar.Seq
+module SS = Zeta.SSeq
 module SA = Zeta.SeqAux
 module T = Zeta.Generic.Thread
 module I = Zeta.Interleave
@@ -18,64 +21,47 @@ module GV = Zeta.GenericVerifier
 (* a global log is a collection of thread-level verifier logs *)
 let vlog (vspec: verifier_spec) = seq (verifier_log vspec)
 
-let thread_log #vspec (gl: vlog vspec) (tid: SA.seq_index gl): T.vlog _ =
+let thread_log_base #vspec (gl: vlog vspec) (tid: SA.seq_index gl): T.vlog _ =
   (tid, S.index gl tid)
 
-let index #vspec (gl: vlog vspec) (i: sseq_index gl) =
+let indexss #vspec (gl: vlog vspec) (i: SS.sseq_index gl) =
   indexss gl i
 
 (* a global log is verifiable if every thread-level log is verifiable *)
 let verifiable #vspec (gl: vlog vspec) =
-  forall (tid: SA.seq_index gl). {:pattern T.verifiable (thread_log gl tid)} T.verifiable (thread_log gl tid)
+  forall (tid: SA.seq_index gl). {:pattern T.verifiable (thread_log_base gl tid)} T.verifiable (thread_log_base gl tid)
 
 let verifiable_log vspec = gl:vlog vspec {verifiable gl}
 
-let idxfn #vspec (#b:eqtype) (tfn: idxfn_t vspec b) (gl: verifiable_log vspec) (ti: sseq_index gl): b
-  = let t,i = ti in
-    let tl = thread_log gl t in
-    tfn tl i
+val lemma_prefix_verifiable (#vspec:_) (gl: verifiable_log vspec) (l: nat{l <= S.length gl})
+  : Lemma (ensures (verifiable (SA.prefix gl l)))
+          [SMTPat (SA.prefix gl l)]
 
-let cond_idxfn #vspec (#b:eqtype) (#f:_) (tfn: cond_idxfn_t #vspec b f)
-  (gl: verifiable_log vspec) (ti: sseq_index gl{idxfn f gl ti})
-  = let t,i = ti in
-    let tl = thread_log gl t in
-    tfn tl i
+let prefix (#vspec:_) (gl: verifiable_log vspec) (l: nat{l <= S.length gl})
+  : gl':verifiable_log vspec {S.length gl' = l}
+  = SA.prefix gl l
 
-(* a theory of filter-map operations using thread idx functions *)
-val filter_map (#vspec:_) (#b:_)
-  (fm: fm_t vspec b)
-  (gl: verifiable_log vspec)
-  : s:sseq b {S.length s = S.length gl}
+let index (#vspec:_) (gl: verifiable_log vspec) (i: SA.seq_index gl)
+  : T.verifiable_log vspec
+  = thread_log_base gl i
 
-(* map an index of the original sequence to the filter-mapped sequence *)
-val filter_map_map (#vspec:_) (#b:_)
-  (fm: fm_t vspec b)
-  (gl: verifiable_log vspec)
-  (ii: sseq_index gl {idxfn fm.f gl ii})
-  : jj: (sseq_index (filter_map fm gl))
-    {indexss (filter_map fm gl) jj == cond_idxfn fm.m gl ii /\
-     fst ii = fst jj}
+let gso (vspec: verifier_spec) : gen_seq_spec = {
+  seq_t = verifiable_log vspec;
+  length = S.length;
+  prefix
+}
 
-(* map an index of the filter-map back to the original sequence *)
-val filter_map_invmap (#vspec:_) (#b:_)
-  (fm: fm_t vspec b)
-  (gl: verifiable_log vspec)
-  (jj: sseq_index (filter_map fm gl))
-  : ii:(sseq_index gl){idxfn fm.f gl ii /\ filter_map_map fm gl ii = jj }
+let gen_sseq (vspec:verifier_spec): gen_sseq = {
+  gso = gso vspec;
+  gsi = T.gen_seq vspec;
+  index
+}
 
-val lemma_filter_map (#vspec:_)  (#b:_)
-  (fm: fm_t vspec b)
-  (gl: verifiable_log vspec)
-  (ii: sseq_index gl {idxfn fm.f gl ii})
-  : Lemma (ensures (let jj = filter_map_map fm gl ii in
-                    ii = filter_map_invmap fm gl jj))
-          [SMTPat (filter_map_map fm gl ii)]
+let idxfn (#vspec:verifier_spec) #b (f: T.idxfn_t vspec b) (gl: verifiable_log vspec) (ii: sseq_index gl)
+  = Zeta.SIdxFn.idxfn #b (gen_sseq vspec) f gl ii
 
-val lemma_filter_map_idx (#vspec:_) (#b:_)
-  (fm: fm_t vspec b)
-  (gl: verifiable_log vspec)
-  (i: SA.seq_index gl)
-  : Lemma (ensures (S.index (filter_map fm gl) i = T.filter_map fm (thread_log gl i)))
+let cond_idxfn (#b:eqtype) (#vspec:verifier_spec) (#f: T.idxfn_t vspec bool)
+  = Zeta.SIdxFn.cond_idxfn #b #(gen_sseq vspec) #f
 
 let clock #vspec = idxfn (T.clock #vspec)
 
@@ -88,7 +74,7 @@ let add_set
     (* filter map specification that filter by AddB? and maps them to blum add elem *)
     let fm = to_fm (T.blum_add_elem #vspec #ep) in
     (* get a seq of seq of blum-add-elems and convert them to multiset *)
-    sseq2mset (filter_map fm gl)
+    sseq2mset (filter_map (gen_sseq vspec) fm gl)
 
 (* blum evict set elements for a given epoch *)
 let evict_set
@@ -97,7 +83,7 @@ let evict_set
   (gl: verifiable_log vspec): mset_ms_hashfn_dom vspec.app
   = let open Zeta.MultiSet.SSeq in
     let fm = to_fm (T.blum_evict_elem #vspec #ep) in
-    sseq2mset (filter_map fm gl)
+    sseq2mset (filter_map (gen_sseq vspec) fm gl)
 
 (* verifiable log property that add- and evict sets are the same *)
 let aems_equal_for_epoch #vspec
@@ -127,4 +113,4 @@ let appfn_call_res
   (ep: epoch)
   (gl: verifiable_log vspec): sseq (Zeta.AppSimulate.appfn_call_res vspec.app)
   = let fm = to_fm (T.appfn_call_res #vspec ep) in
-    filter_map fm gl
+    filter_map (gen_sseq vspec) fm gl
