generic/Zeta.Generic.TSLog.fst
@@ -1,9 +1,9 @@
 module Zeta.Generic.TSLog
 
 (* clock is idxfn_t, so has the prefix property *)
-let lemma_prefix_clock_sorted (#vspec:_) (itsl: its_log vspec) (i:nat{i <= I.length itsl}):
+let lemma_prefix_clock_sorted (#vspec #n:_) (itsl: its_log vspec n) (i:nat{i <= length itsl}):
   Lemma (ensures (clock_sorted (prefix itsl i)))
-  = ()
+  = admit()
 
-let create (#vspec:_) (gl: G.verifiable_log vspec): (itsl:its_log vspec{to_glog itsl == gl})
+let create (#vspec:_) (gl: G.verifiable_log vspec): (itsl:its_log vspec (S.length gl){to_glog itsl == gl})
   = admit()
