generic/Zeta.Generic.TSLog.fsti
@@ -11,14 +11,16 @@ open Zeta.Generic.Interleave
 
 module I = Zeta.Interleave
 module G = Zeta.Generic.Global
+module S = FStar.Seq
+module SA = Zeta.SeqAux
 
-let clock_sorted (#vspec:_) (il: verifiable_log vspec) =
-  forall (i j: I.seq_index il). i <= j ==> clock il i `ts_leq` clock il j
+let clock_sorted (#vspec:_) (#n:_) (il: verifiable_log vspec n) =
+  forall (i j: seq_index il). i <= j ==> clock il i `ts_leq` clock il j
 
-let its_log vspec = il:verifiable_log vspec{clock_sorted il}
+let its_log vspec n = il:verifiable_log vspec n{clock_sorted il}
 
-val lemma_prefix_clock_sorted (#vspec:_) (itsl: its_log vspec) (i:nat{i <= I.length itsl}):
+val lemma_prefix_clock_sorted (#vspec #n:_) (itsl: its_log vspec n) (i:nat{i <= length itsl}):
   Lemma (ensures (clock_sorted (prefix itsl i)))
-        [SMTPat (I.prefix itsl i)]
+        [SMTPat (prefix itsl i)]
 
-val create (#vspec:_) (gl: G.verifiable_log vspec): (itsl:its_log vspec{to_glog itsl == gl})
+val create (#vspec:_) (gl: G.verifiable_log vspec): (itsl:its_log vspec (S.length gl){to_glog itsl == gl})
