utils/Zeta.IdxFn.fsti
@@ -130,6 +130,9 @@ type fm_t (gs:_) (b:eqtype) =
   | FM: f: idxfn_t gs bool   ->
         m: cond_idxfn_t b f -> fm_t gs b
 
+let to_fm (#gs:_) (#b:eqtype) (#f:idxfn_t gs bool) (m: cond_idxfn_t b f)
+  = FM f m
+
 (* apply the filter fm.f on s to get a filtered sequence; apply fm.m on each element to get the result *)
 let filter_map (#gs #b:_)
   (fm: fm_t gs b)
